Cslib.lean
@@ -32,6 +32,9 @@ public import Cslib.Computability.Languages.RegularLanguage
 public import Cslib.Computability.Machines.MultiTapeTuring.AddRoutine
 public import Cslib.Computability.Machines.MultiTapeTuring.Basic
 public import Cslib.Computability.Machines.MultiTapeTuring.CopyRoutine
+public import Cslib.Computability.Machines.MultiTapeTuring.DecRoutine
+public import Cslib.Computability.Machines.MultiTapeTuring.DuplicateRoutine
+public import Cslib.Computability.Machines.MultiTapeTuring.Encoding
 public import Cslib.Computability.Machines.MultiTapeTuring.EqualRoutine
 public import Cslib.Computability.Machines.MultiTapeTuring.GraphReachability
 public import Cslib.Computability.Machines.MultiTapeTuring.HeadStats
@@ -43,7 +46,9 @@ public import Cslib.Computability.Machines.MultiTapeTuring.MoveRoutine
 public import Cslib.Computability.Machines.MultiTapeTuring.MulRoutine
 public import Cslib.Computability.Machines.MultiTapeTuring.PopRoutine
 public import Cslib.Computability.Machines.MultiTapeTuring.PushRoutine
+public import Cslib.Computability.Machines.MultiTapeTuring.Satisfiability
 public import Cslib.Computability.Machines.MultiTapeTuring.SequentialCombinator
+public import Cslib.Computability.Machines.MultiTapeTuring.StructuralMachines
 public import Cslib.Computability.Machines.MultiTapeTuring.SuccRoutine
 public import Cslib.Computability.Machines.MultiTapeTuring.TapeExtension
 public import Cslib.Computability.Machines.MultiTapeTuring.WhileCombinator
